NonEmpty.v
@@ -24,3 +24,9 @@ Fixpoint NE_tl {a} (ne : NonEmpty a) : a :=
     | NE_Sing x => x
     | NE_Cons x xs => NE_tl xs
   end.
+
+Fixpoint NE_fold_left {a b : Set} (f : a -> b -> a) (ne : NonEmpty b) (z : a) : a :=
+  match ne with
+    | NE_Sing x => f z x
+    | NE_Cons x xs => NE_fold_left f xs (f z x)
+  end.
