SSMorph.v
@@ -1,0 +1,173 @@
+Require Import Coq.Program.Tactics.
+Require Import Coq.Structures.Orders.
+Require Import Fin.
+Require Import Interval.
+Require Import Lib.
+Require Import ScanState.
+
+Generalizable All Variables.
+
+Module MSSMorph (M : Machine).
+Include MScanState M.
+
+(** ** SSMorph *)
+
+(** A [SSMorph] is a relation describe a lawful transition between two
+    states.  It is a [PreOrder] relation. *)
+
+Record SSMorph (sd1 sd2 : ScanStateDesc) : Prop := {
+    next_interval_increases : nextInterval sd1     <= nextInterval sd2;
+    total_extent_decreases  : unhandledExtent sd2  <= unhandledExtent sd1;
+    handled_count_increases : length (handled sd1) <= length (handled sd2)
+}.
+
+Arguments next_interval_increases [sd1 sd2] _.
+Arguments total_extent_decreases  [sd1 sd2] _.
+Arguments handled_count_increases [sd1 sd2] _.
+
+Definition newSSMorph (s : ScanStateDesc) : SSMorph s s.
+Proof. constructor; auto. Defined.
+
+Program Instance SSMorph_PO : PreOrder SSMorph.
+Obligation 1. constructor; auto. Defined.
+Obligation 2.
+  constructor; destruct H; destruct H0.
+  transitivity (nextInterval y); auto.
+  transitivity (unhandledExtent y); auto.
+  transitivity (length (handled y)); auto.
+Defined.
+
+Record SSMorphLen (sd1 sd2 : ScanStateDesc) : Prop := {
+    len_is_SSMorph :> SSMorph sd1 sd2;
+
+    unhandled_nonempty :
+      length (unhandled sd1) > 0 -> length (unhandled sd2) > 0
+}.
+
+Definition newSSMorphLen (s : ScanStateDesc) : SSMorphLen s s.
+Proof. intros. constructor; auto. constructor; auto. Defined.
+
+Record SSMorphSt (sd1 sd2 : ScanStateDesc) : Prop := {
+    st_is_SSMorph :> SSMorph sd1 sd2;
+
+    total_extent_measurably_decreases :
+      unhandledExtent sd2 < unhandledExtent sd1
+}.
+
+Program Instance SSMorphSt_Trans : Transitive SSMorphSt.
+Obligation 1.
+  constructor.
+    destruct H. destruct H0.
+    transitivity y; assumption.
+  inversion H. inversion H0.
+  destruct total_extent_measurably_decreases1. omega.
+  destruct total_extent_measurably_decreases0. omega.
+  right. omega.
+Qed.
+
+Record SSMorphStLen (sd1 sd2 : ScanStateDesc) : Prop := {
+    stlen_is_SSMorphLen :> SSMorphLen sd1 sd2;
+    stlen_is_SSMorphSt  :> SSMorphSt sd1 sd2
+}.
+
+Lemma ScanState_unhandledExtent_nonzero `(st : ScanState sd) :
+  length (unhandled sd) > 0 <-> unhandledExtent sd > 0.
+Proof.
+  intros.
+  ScanState_cases (induction st) Case; simpl in *.
+  - Case "ScanState_nil".
+    split; intros; inversion H.
+  - Case "ScanState_newUnhandled".
+    pose (Interval_extent_nonzero i).
+    destruct unh eqn:Heqe;
+    unfold unhandledExtent; simpl.
+      split; intros; try cmp_reflexive; auto.
+    destruct l eqn:Heqe2; simpl.
+      split; intros; try cmp_reflexive; auto. omega.
+    split; intros.
+      apply fold_gt.
+      cmp_reflexive. omega.
+    apply Gt.gt_Sn_O.
+  - Case "ScanState_moveUnhandledToActive".
+    apply ScanState_unhandledExtent in st.
+    rename st into i. simpl in *.
+    destruct unh eqn:Heqe.
+      split; intros. inversion H. auto.
+    unfold unhandledExtent; simpl.
+    destruct l eqn:Heqe2; simpl.
+      split; intros.
+      apply Interval_extent_nonzero.
+      auto.
+    split; intros.
+      apply fold_gt.
+      pose (Interval_extent_nonzero (projT2 (geti f))).
+      omega.
+    omega.
+  - Case "ScanState_moveActiveToInactive".  apply IHst.
+  - Case "ScanState_moveActiveToHandled".   apply IHst.
+  - Case "ScanState_moveInactiveToActive".  apply IHst.
+  - Case "ScanState_moveInactiveToHandled". apply IHst.
+Qed.
+
+Definition moveActiveToHandled `(st : ScanState sd) (x : IntervalId sd)
+  (H : In x (active sd)) : NextScanState (SSMorphLen sd).
+Proof.
+  pose (ScanState_moveActiveToInactive sd x st H). eexists. apply s.
+  destruct sd. simpl.
+  rapply Build_SSMorphLen; auto.
+  rapply Build_SSMorph; auto.
+Defined.
+
+Definition moveActiveToInactive `(st : ScanState sd) (x : IntervalId sd)
+  (H : In x (active sd)) : NextScanState (SSMorphLen sd).
+Proof.
+  pose (ScanState_moveActiveToInactive sd x st H). eexists. apply s.
+  destruct sd. simpl.
+  rapply Build_SSMorphLen; auto.
+  rapply Build_SSMorph; auto.
+Defined.
+
+Definition moveInactiveToActive `(st : ScanState sd) (x : IntervalId sd)
+  (H : In x (inactive sd)) : NextScanState (SSMorphLen sd).
+Proof.
+  pose (ScanState_moveInactiveToActive sd x st H). eexists. apply s.
+  destruct sd. simpl.
+  rapply Build_SSMorphLen; auto.
+  rapply Build_SSMorph; auto.
+Defined.
+
+Definition moveInactiveToHandled `(st : ScanState sd) (x : IntervalId sd)
+  (H : In x (inactive sd)) : NextScanState (SSMorphLen sd).
+Proof.
+  pose (ScanState_moveInactiveToHandled sd x st H). eexists. apply s.
+  destruct sd. simpl.
+  rapply Build_SSMorphLen; auto.
+  rapply Build_SSMorph; auto.
+  apply Le.le_n_Sn.
+Defined.
+
+Definition moveUnhandledToActive `(cur : ScanStateCursor sd) (reg : PhysReg)
+  : NextState cur SSMorphSt.
+Proof.
+  destruct cur. destruct sd.
+  destruct unhandled0; simpl in *. omega.
+  pose (ScanState_moveUnhandledToActive nextInterval0 unhandled0
+          (* unhsort *)
+          active0 inactive0 handled0 getInterval0 assignments0
+          getFixedInterval0 i reg lists_are_unique0).
+  eexists. apply s. apply curState0.
+  pose (unhandledExtent_cons nextInterval0 i unhandled0 getInterval0
+         (fun i0 : fin nextInterval0 =>
+            if cmp_eq_dec i0 i
+            then Some reg
+            else assignments0 i0) assignments0 getFixedInterval0
+         (i :: active0) active0 inactive0 inactive0 handled0 handled0
+         (move_unhandled_to_active _ i unhandled0 active0 inactive0 handled0
+            lists_are_unique0) lists_are_unique0)
+    as ue_cons.
+  rapply Build_SSMorphSt; auto.
+  rapply Build_SSMorph; auto.
+  apply (Lt.lt_le_weak _ _ ue_cons).
+Defined.
+
+End MSSMorph.
